Two new files are added: multiwordScript and arm_multiwordScript. These contain proofs of algorithms and ARM implementations of arithmetic operations (including Montgomery multiplication) over lists of words that represent large natural numbers.
The other changes are various small changes that have accumulated
over the last few months.

examples/elliptic/sep/arm_progLib.sig
@@ -15,6 +15,7 @@ sig
 
     val PRE_CONV_RULE       : conv -> thm -> thm   
     val POST1_CONV_RULE     : conv -> thm -> thm
+    val POST2_CONV_RULE     : conv -> thm -> thm
     val POST_CONV_RULE      : conv -> thm -> thm
 
     val PRE_MOVE_STAR       : term frag list -> term frag list -> thm -> thm   
@@ -29,6 +30,9 @@ sig
     val MATCH_COMPOSE       : thm -> thm -> thm
     val ARRANGE_COMPOSE     : thm -> thm -> thm
     val FRAME_COMPOSE       : thm -> thm -> thm
+    val MOVE_COMPOSE        : thm -> thm -> 
+                              term frag list -> term frag list -> 
+                              term frag list -> term frag list -> thm
 
     val HIDE_PRE            : thm -> thm
     val HIDE_POST1          : thm -> thm
@@ -36,9 +40,19 @@ sig
     val HIDE_STATUS         : thm -> thm
     val EXISTS_PRE          : term frag list -> thm -> thm
 
+    val MOVE_PRE            : term frag list -> thm -> thm
+    val MOVE_POST           : term frag list -> thm -> thm
+    val MOVE_POST1          : term frag list -> thm -> thm
+    val MOVE_POST2          : term frag list -> thm -> thm
+
+    val AUTO_HIDE_PRE       : (term frag list) list -> thm -> thm
+    val AUTO_HIDE_POST1     : (term frag list) list -> thm -> thm
+    val AUTO_HIDE_POST2     : (term frag list) list -> thm -> thm
+
     val AUTO_PRE_HIDE_STATUS   : thm -> thm
     val AUTO_POST1_HIDE_STATUS : thm -> thm
     val AUTO_POST_HIDE_STATUS  : thm -> thm
+    val AUTO_HIDE_STATUS       : thm -> thm
 
     val APP_BASIC_FRAME     : thm -> thm
     val APP_FRAME           : term frag list -> thm -> thm
@@ -58,20 +72,37 @@ sig
     val APP_PART_WEAKEN_TERM     : thm -> term frag list -> term 
     val APP_PART_WEAKEN          : thm -> term frag list -> tactic -> thm 
 
+    val SPEC_STRENGTHEN     : thm -> term frag list -> thm
+    val SPEC_WEAKEN1        : thm -> term frag list -> thm
+    val SPEC_WEAKEN         : thm -> term frag list -> thm
+    val SEP_IMP_RULE        : (term -> thm) -> thm -> thm
+
     val ALIGN_VARS          : string list -> thm -> thm
+ 
+    val MATCH_INST1         : term frag list list -> thm -> thm -> thm
+    val MATCH_INST          : term frag list list -> thm -> thm -> thm
+     
+    val ARM_PROG_CLOSE_LOOP : thm -> thm
+    val EXTRACT_CODE        : thm -> thm
+    val ABSORB_POST         : thm -> thm
 
     val PAT_DISCH           : term -> thm -> thm
     val PAIR_GEN            : string -> term frag list -> thm -> thm
+    val QGENL               : term frag list list -> thm -> thm
+    val INST_LDM_STM        : bool -> term frag list -> term frag list -> 
+                              thm -> term frag list -> thm
 
     val show_enc            : bool ref
     val show_code           : bool ref
-    val show_code_verbosely : bool ref
  
     val pp_enc              : unit -> unit
 
     (* experimental proof-producing functions *)
  
     val print_compositions  : (thm * string) list -> string -> string -> unit   
+
+    val make_spec           : string list -> unit
+    val make_spec'          : (string * bool) list -> unit
 
     val compose_progs       : string list -> string -> string -> unit
     val compose_progs'      : (string * bool) list -> string -> string -> unit
